Makefile
@@ -157,7 +157,7 @@ POLCERT_SRC = Base.v Convert.v \
   Extractor.v PrepareCodegen.v StrengthenDomain.v \
   OpenScop.v OpenScopAST.v PolyBase.v PolyLang.v \
   SelectionSort.v StablePermut.v CState.v AffineValidator.v \
-  TransformContract.v StateView.v ViewPipeline.v StorageWitness.v SourceNoAliasWitness.v FramePreservationWitness.v FramePreservationValidator.v StateObservation.v LayoutWitness.v \
+  TransformContract.v StateView.v ViewPipeline.v StorageWitness.v CellView.v SourceNoAliasWitness.v FramePreservationWitness.v FramePreservationValidator.v StateObservation.v LayoutWitness.v \
   LayoutRemapValidator.v PrivateStorageWitness.v PrivateBoundaryWitness.v PaddingLayoutWitness.v LayoutValueWitness.v PaddingLayoutValidator.v PrivateStorageValidator.v CopyProtocolWitness.v CopyCommitWitness.v CopyInstanceWitness.v CopyMappingWitness.v \
   ScalarPromotionWitness.v ScalarPromotionValueWitness.v ScalarPromotionValidator.v CopyProtocolValueWitness.v CopyProtocolValidator.v ScratchpadCopyValidator.v ReuseConflictWitness.v LifetimeConflictWitness.v ReuseValueWitness.v StorageCompatibilityWitness.v InterArrayReuseWitness.v InterArrayReuseValidator.v ReuseStateView.v StorageBoundaryView.v ReuseConflictValidator.v InstanceProjectionWitness.v \
   InstanceProjectionValidator.v OverlapClosureWitness.v OverlapTilingValidator.v VersionCommitWitness.v VersionCommitValueWitness.v VersionCommitValidator.v \
